Rename [install] to [wrap] (and related names).

coq-osiris/theories/semantics/code.v
@@ -58,7 +58,7 @@ Definition eff := val.
 
    The result is a value (or an exception). *)
 
-(* [CInstall (deep, k, η, bs)] retrieves the continuation stored at [k] and installs
+(* [CWrap (deep, k, η, bs)] retrieves the continuation stored at [k] and installs
     a handler around it at a new location.
 
     The handler is given by [bs] (list of branches), and is evaluated with
@@ -73,7 +73,7 @@ Inductive code : Type → Type → Type → Type :=
 | CStore : code (loc * val) unit exn
 | CPerf  : code eff val exn
 | CResume : code (loc * outcome2 val exn) val exn
-| CInstall : code (bool * loc * env * handler) loc exn
+| CWrap : code (bool * loc * env * handler) loc exn
 .
 
 (* ------------------------------------------------------------------------ *)
@@ -110,11 +110,11 @@ Definition please_eval η e :=
 Definition perform (v : eff) : microvx :=
   stop CPerf v.
 
-(* The computation [install η k bs] installs a handler [bs] for the continuation
+(* The computation [wrap η k bs] installs a handler [bs] for the continuation
   stored at [k], and returns a new location which stores this installation. *)
 
-Definition install deep k η bs : micro loc exn :=
-  stop CInstall (deep, k, η, bs).
+Definition wrap deep k η bs : micro loc exn :=
+  stop CWrap (deep, k, η, bs).
 
 Definition resume (l : loc) (o : outcome2 val exn) :=
   stop CResume (l, o).
