coq-osiris/theories/program_logic/basic_rules.v
@@ -735,24 +735,24 @@ Section ewp_rules.
     iFrame.
   Qed.
 
-  (* [CInstall]. *)
+  (* [CWrap]. *)
 
   (* Installing a handler with branches [bs] on top of a continuation
      that is located in the store at location [l]. *)
 
-  Lemma ewp_install_deep {B Y} E l η bs (k: _ -> micro B Y) φ ψ :
+  Lemma ewp_wrap_deep {B Y} E l η bs (k: _ -> micro B Y) φ ψ :
     (∀ l',
       l'↦
         (K (λ o, Handle (stop CResume (l, o)) (wrap_eval_branches η bs))) -∗
      ▷ EWP (continue k l') @ E <| ψ |> {{ φ }}) -∗
-    EWP (Stop CInstall (true, l, η, bs) k) @ E <| ψ |> {{ φ }}.
+    EWP (Stop CWrap (true, l, η, bs) k) @ E <| ψ |> {{ φ }}.
   Proof.
     iIntros "Hwp".
     ewp_unfold_head; intro_state; ewp_mask_intro "Hmod".
     construct_wp_nonret.
 
     (* The reduction step must be a successful step. *)
-    eapply invert_step_install_deep in Hstep as (l' & ? & ? & ?); subst.
+    eapply invert_step_wrap_deep in Hstep as (l' & ? & ? & ?); subst.
 
     (* Allocate a new location in the heap. *)
     iMod (gen_heap.gen_heap_alloc with "Hsi") as "(Hsi & Hl' & _)"; first done.
@@ -762,19 +762,19 @@ Section ewp_rules.
     done.
   Qed.
 
-  Lemma ewp_install_shallow {B Y} E l η bs (k: _ -> micro B Y) φ ψ :
+  Lemma ewp_wrap_shallow {B Y} E l η bs (k: _ -> micro B Y) φ ψ :
     (∀ l',
       l'↦
         (K (λ o, Handle (stop CResume (l, o)) (λ o, shallow_match η o bs bs))) -∗
      ▷ EWP (continue k l') @ E <| ψ |> {{ φ }}) -∗
-    EWP (Stop CInstall (false, l, η, bs) k) @ E <| ψ |> {{ φ }}.
+    EWP (Stop CWrap (false, l, η, bs) k) @ E <| ψ |> {{ φ }}.
   Proof.
     iIntros "Hwp".
     ewp_unfold_head; intro_state; ewp_mask_intro "Hmod".
     construct_wp_nonret.
 
     (* The reduction step must be a successful step. *)
-    eapply invert_step_install_shallow in Hstep as (l' & ? & ? & ?); subst.
+    eapply invert_step_wrap_shallow in Hstep as (l' & ? & ? & ?); subst.
 
     (* Allocate a new location in the heap. *)
     iMod (gen_heap.gen_heap_alloc with "Hsi") as "(Hsi & Hl' & _)"; first done.
